\documentclass{article}\usepackage{breqn}\begin{document}M = 2, n = 1:\newline\newline Original equation:\begin{dmath}  +  3f_{-1}f_{0}^2  +  3f_{-1}^2f_{1}  +  6f_{-2}f_{0}f_{1}  +  6f_{-2}f_{-1}f_{2}
 = 0\end{dmath}Equivalent equation, where $f_{-j}=\overline{f_j}$:\begin{dmath}3 f_{0}^{2} \overline{f_{1}} + 6 f_{0} f_{1} \overline{f_{2}} + 3 f_{1} \overline{f_{1}}^{2} + 6 f_{2} \overline{f_{1}} \overline{f_{2}} = 0\end{dmath}All possible solutions:\begin{dmath}\left \{ f_{1} : 0\right \}\end{dmath}
Time elapsed: 0.7640247344970703 seconds\end{document}